Ass12 completed

sf/Assignment12_05.v
@@ -13,32 +13,47 @@ Require Export Assignment12_04.
 *)
 
 Definition halve : tm :=
-  FILL_IN_HERE.
+tfix (tabs Halve (TArrow TNat TNat)
+       (tabs X TNat
+         (tif0 (tvar X) (tnat 0)
+           (tif0 (tpred (tvar X)) (tnat 0)
+             (tsucc (tapp (tvar Halve) (tpred (tpred (tvar X))))))))).
+
+Hint Unfold halve.
 
 Example halve_type: empty |- halve \in TArrow TNat TNat.
-Proof.
-  (* unfold halve; eauto 10. *)
-  exact FILL_IN_HERE.
-Qed.
+Proof. unfold halve ; eauto 10. Qed.
 
 Example halve_10: tapp halve (tnat 10) ==>* tnat 5.
-Proof.
-  (* unfold halve; normalize. *)
-  exact FILL_IN_HERE.
-Qed.
+Proof. unfold halve ; normalize. Qed.
 
 Example halve_11: tapp halve (tnat 11) ==>* tnat 5.
-Proof.
-  (* unfold halve; normalize. *)
-  exact FILL_IN_HERE.
-Qed.
+Proof. unfold halve; normalize. Qed.
 
+
+Lemma halve_supp: forall t t', t ==>* t' -> (tsucc t) ==>* (tsucc t').
+Proof.
+  intros. induction H. constructor. assert (tsucc x ==> tsucc y).
+  constructor. assumption. apply multi_step with (tsucc y); assumption.
+Qed.
 
 Theorem halve_correct: forall n,
    tapp halve (tnat (n+n)) ==>* tnat n.
 Proof.
-  exact FILL_IN_HERE.
+  intros. induction n.
+  - simpl. unfold halve. normalize.
+  - assert (tapp halve (tnat (S n + S n)) ==>* tsucc (tapp halve (tnat (n + n)))).
+    + assert (S n + S n = S (S (n + n))). omega. rewrite H.  
+      unfold halve. eapply multi_step. apply ST_AppFix. eauto. eauto.
+      eapply multi_step. apply ST_App1. eauto. 
+      repeat (eapply multi_step; compute; eauto).
+    + apply multi_trans with (y:= tsucc (tapp halve (tnat (n + n)))).
+      assumption. assert (tsucc (tapp halve (tnat (n + n))) ==>* tsucc (tnat n)).
+      apply halve_supp. assumption. apply multi_trans with (y:= tsucc (tnat n)).
+      assumption. apply multi_step with (tnat (S n)). constructor. eauto.
 Qed.
+
+
 
 (*-- Check --*)
 
