sf/Assignment12_04.v
@@ -7,11 +7,11 @@ Corollary soundness : forall t t' T,
   t ==>* t' ->
   ~(stuck t').
 Proof.
-
-
-
-
-  exact FILL_IN_HERE.
+  intros. intros contra. unfold stuck in contra. unfold normal_form in contra.
+  inversion contra. unfold not in H1. unfold not in H2. induction H0.
+  - apply progress in H. inversion H. auto. auto. 
+  - apply preservation with (t' := y) in H. apply IHmulti in H ; try auto.
+    assumption.
 Qed.
 
 (*-- Check --*)
@@ -19,4 +19,3 @@ Check soundness : forall t t' T,
   empty |- t \in T -> 
   t ==>* t' ->
   ~(stuck t').
-
