sf/Assignment12_06.v
@@ -2,13 +2,82 @@ Require Export Assignment12_05.
 
 (* problem #06: 10 points *)
 
+Theorem MoreStlc_value_is_nf: forall v t,
+  value v -> v ==> t -> False.
+Proof with eauto.
+  intros; generalize dependent t; assert (normal_form step v)...
+  unfold normal_form; intros; induction H; intros contra; destruct contra;
+  try solve by inversion; try inversion H0; try inversion H1; subst...
+Qed.
+
+Hint Resolve MoreStlc_value_is_nf.
+
+Theorem MoreStlc_deterministic:
+  deterministic step.
+Proof with eauto.
+  unfold deterministic; intros; generalize dependent y2;
+  induction H as [| |? ? ? ? P| | | | | |? ? ? ? P| | | | | |? ? ? ? P| |? ? ? P|
+  |? ? ? P| | | | | | | | |? ? ? ? P| | | ? ? ? ? ? ? P| |? ? ? P]; intros;
+  inversion H0; subst; try solve by inversion;
+  try replace t0'0 with t0';
+  try replace t1'0 with t1';
+  try replace t2'0 with t2';
+  eauto; exfalso...
+Qed.
+
+Lemma determ_supp: forall t t1 t2:tm, t ==> t1 -> t ==> t2 -> t1 = t2.
+Proof.
+  apply MoreStlc_deterministic.
+Qed.
+
+
+Lemma looping: forall t q1 q2 q3, q1 ==>* t -> q1 ==> q2 -> q2 ==> q3 -> q3 ==> q1 -> 
+                (t = q1 \/ t = q2 \/ t = q3).
+Proof.
+  intros t q1 q2 q3 H. generalize dependent q2. generalize dependent q3.
+  induction H. intros. left. auto.
+  intros. assert (y = q2). apply determ_supp with (t:= x) ; assumption. subst y.
+  assert (z = q2 \/ z = q3 \/ z = x). apply IHmulti ; assumption.
+  destruct H4. right. left. assumption. destruct H4. right. right. assumption.
+  left. assumption.
+Qed.
+
 Theorem tloop_diverges:
   ~ exists t, tapp tloop (tnat 0) ==>* t /\ normal_form step t.
 Proof.
-  exact FILL_IN_HERE.
+  intros contra. inversion contra. inversion H. unfold normal_form in H1.
+  unfold not in H1. assert (value tloop). unfold tloop. eauto. 
+  remember (tabs Loop (TArrow TNat TNat) (tabs X TNat (tapp (tvar Loop) (tvar X)))) as F1.
+  assert (value F1). rewrite HeqF1. eauto. remember (tnat 0) as v1. assert (value v1). rewrite Heqv1. eauto.
+  unfold tloop in H0. rewrite <- HeqF1 in H0.
+  assert (tapp (tfix F1) v1 ==> tapp (tapp F1 (tfix F1)) v1). apply ST_AppFix ; assumption. 
+  assert (forall t', tapp (tfix F1) v1 ==> t' -> t' = tapp (tapp F1 (tfix F1)) v1). 
+  intros. apply determ_supp with (t:= tapp (tfix F1) v1) ; assumption.
+  assert (value (tfix F1)). rewrite HeqF1. eauto.
+  remember (tfix F1) as v2. remember (tabs X TNat (tapp (tvar Loop) (tvar X))) as t12.
+  assert (tapp (tapp F1 v2) v1 ==> tapp ([Loop := v2]t12) v1). rewrite HeqF1. apply ST_App1.
+  apply ST_AppAbs. assumption.
+  assert (forall t', tapp (tapp F1 v2) v1 ==> t' -> t' = tapp ([Loop := v2]t12) v1). intros.
+  apply determ_supp with (t:= tapp (tapp F1 v2) v1) ; assumption.
+  assert (tapp ([Loop := v2]t12) v1 = tapp (tabs X TNat (tapp v2 (tvar X)))v1). 
+  rewrite Heqt12. simpl. reflexivity. rewrite H10 in H9.
+  assert (value (tabs X TNat (tapp v2 (tvar X)))). eauto.
+  assert (tapp (tabs X TNat (tapp v2 (tvar X))) v1 ==> [X := v1](tapp v2 (tvar X))). eauto.
+  assert (forall t', tapp (tabs X TNat (tapp v2 (tvar X))) v1 ==> t' -> t' = [X := v1](tapp v2 (tvar X))).
+  intros. apply determ_supp with (t:= tapp (tabs X TNat (tapp v2 (tvar X))) v1) ; assumption.
+  assert ([X := v1]tapp v2 (tvar X) = tapp tloop v1). rewrite Heqv1. rewrite Heqv2. simpl. rewrite HeqF1.
+  rewrite Heqt12. auto. assert (tapp tloop v1 = tapp v2 v1). rewrite Heqv1. rewrite Heqv2. unfold tloop.
+  rewrite HeqF1. rewrite Heqt12. reflexivity. rewrite <- H15 in H6. rewrite <-H15 in H5.
+  clear H3 H4 H7 H2. remember (tapp tloop v1) as q1. remember (tapp (tapp F1 v2) v1) as q2.
+  rewrite H10 in H8. remember (tapp (tabs X TNat (tapp v2 (tvar X))) v1) as q3.
+  rewrite H14 in H12. rewrite H14 in H13. clear H10 H14. clear HeqF1 Heqt12 H0. inversion H. clear H2.
+  { assert (x = q1 \/ x = q2 \/ x = q3). apply looping; assumption.
+    destruct H2. subst x. eauto. 
+    destruct H2. subst x. eauto.
+    subst x. eauto.
+  } 
 Qed.
 
 (*-- Check --*)
 Check tloop_diverges:
   ~ exists t, tapp tloop (tnat 0) ==>* t /\ normal_form step t.
-
